BB4 extraction and slight renamings in BB5 and updated extraction building script

CoqBB5/BB4/BB4_Extraction.v
@@ -1,30 +1,17 @@
-From CoqBB5 Require Import TNF.
-From CoqBB5 Require Import BB5_Statement.
-From CoqBB5 Require Import BB5_Deciders_Generic.
-From CoqBB5 Require Import BB5_Deciders_Pipeline.
-From CoqBB5 Require Import BB5_TNF_Enumeration.
-
-
-(** In the OCaml extraction, we do not decompose the TNF tree in several roots (see TNF_Roots/) as this is used only to parallelise the proof. 
-
-The following definitions encompass the entire TNF tree in 200 batches of at most 2^20 machines,
-as done before the proof was parallelised, see:
-
-- https://github.com/ccz181078/Coq-BB5/blob/2a4445600061cc21c05f7390a790694972996bad/BB52Theorem.v#L18286
-- https://github.com/ccz181078/Coq-BB5/blob/2a4445600061cc21c05f7390a790694972996bad/BB52Theorem.v#L18693
-**)
-Definition q_0 := root_q_upd1_simplified.
-Definition q_suc:SearchQueue->SearchQueue := (fun x => SearchQueue_upds x decider_all 20).
-Definition q_200 := Nat.iter 200 q_suc q_0.
+From CoqBB4 Require Import TNF.
+From CoqBB4 Require Import BB4_Statement.
+From CoqBB4 Require Import BB4_Deciders_Generic.
+From CoqBB4 Require Import BB4_Deciders_Pipeline.
+From CoqBB4 Require Import BB4_TNF_Enumeration.
 
 Require Import Extraction.
 Require Import ExtrOcamlBasic ExtrOcamlNatBigInt ExtrOcamlString.
 
-(* Opposite to makeTM, transforms TMs to more convenient representation such as "BR0 BL0 CL1 DR1 DR1 EL0 AL1 DR0 DR1 HR1". *)
+(* Opposite to makeTM, transforms TMs to more convenient representation such as "BR0 BL0 BL1 BR1 AR1 AL0 AL1 None". *)
 Definition unmakeTM : TM Σ ->
-                      (option (Trans Σ) * option (Trans Σ) * option (Trans Σ) * option (Trans Σ) * option (Trans Σ) * option (Trans Σ) * option (Trans Σ) * option (Trans Σ) * option (Trans Σ) * option (Trans Σ)) :=
+                      (option (Trans Σ) * option (Trans Σ) * option (Trans Σ) * option (Trans Σ) * option (Trans Σ) * option (Trans Σ) * option (Trans Σ) * option (Trans Σ)) :=
   fun f =>
-    (f St0 Σ0, f St0 Σ1, f St1 Σ0, f St1 Σ1, f St2 Σ0, f St2 Σ1, f St3 Σ0, f St3 Σ1, f St4 Σ0, f St4 Σ1).
+    (f St0 Σ0, f St0 Σ1, f St1 Σ0, f St1 Σ1, f St2 Σ0, f St2 Σ1, f St3 Σ0, f St3 Σ1).
 
 Require Import String.
 Open Scope string.
@@ -48,8 +35,9 @@ Definition dirToString : Dir -> string :=
 
 Definition stateToString : St -> string :=
   fun s => match s with
-        | St0 => "A" | St1 => "B"| St2 => "C"| St3 => "D"| St4 => "E"
+        | St0 => "A" | St1 => "B"| St2 => "C"| St3 => "D"
         end.
+
 
 Definition transToString : option (Trans Σ) -> string :=
   fun o =>
@@ -58,23 +46,22 @@ Definition transToString : option (Trans Σ) -> string :=
     | Some (Build_Trans _ nxt dir out) => outToString out ++ dirToString dir ++ stateToString nxt
     end.
 
-Definition tmToString : (option (Trans Σ) * option (Trans Σ) * option (Trans Σ) * option (Trans Σ) * option (Trans Σ) * option (Trans Σ) * option (Trans Σ) * option (Trans Σ) * option (Trans Σ) * option (Trans Σ)) -> string :=
-  fun '(A0, A1, B0, B1, C0, C1, D0, D1, E0, E1) =>
+Definition tmToString : (option (Trans Σ) * option (Trans Σ) * option (Trans Σ) * option (Trans Σ) * option (Trans Σ) * option (Trans Σ) * option (Trans Σ) * option (Trans Σ)) -> string :=
+  fun '(A0, A1, B0, B1, C0, C1, D0, D1) =>
     transToString A0 ++ transToString A1 ++ "_" ++
       transToString B0 ++ transToString B1 ++ "_" ++
       transToString C0 ++ transToString C1 ++ "_" ++
-      transToString D0 ++ transToString D1 ++ "_" ++
-      transToString E0 ++ transToString E1.
+      transToString D0 ++ transToString D1.
 
 (** Converting decider identifiers to strings
 **)
 Definition deciderIdentifierToString : DeciderIdentifier -> string :=
   fun decider_id =>
     match decider_id with
-    | DECIDER_NIL => "DECIDER_NIL" 
-    | LOOP1_params_130 => "LOOP1_params_130"
+    | DECIDER_NIL => "DECIDER_NIL"
+    | LOOP1_params_107 => "LOOP1_params_107"
     | NGRAM_CPS_IMPL2_params_1_1_100 => "NGRAM_CPS_IMPL2_params_1_1_100"
-    | NGRAM_CPS_IMPL2_params_2_2_200  => "NGRAM_CPS_IMPL2_params_2_2_200"
+    | NGRAM_CPS_IMPL2_params_2_2_200 => "NGRAM_CPS_IMPL2_params_2_2_200"
     | NGRAM_CPS_IMPL2_params_3_3_400 => "NGRAM_CPS_IMPL2_params_3_3_400"
     | NGRAM_CPS_IMPL1_params_2_2_2_1600 => "NGRAM_CPS_IMPL1_params_2_2_2_1600"
     | NGRAM_CPS_IMPL1_params_2_3_3_1600 => "NGRAM_CPS_IMPL1_params_2_3_3_1600"
@@ -85,14 +72,15 @@ Definition deciderIdentifierToString : DeciderIdentifier -> string :=
     | NGRAM_CPS_IMPL1_params_6_3_3_3200 => "NGRAM_CPS_IMPL1_params_6_3_3_3200"
     | NGRAM_CPS_IMPL1_params_8_2_2_1600 => "NGRAM_CPS_IMPL1_params_8_2_2_1600"
     | NGRAM_CPS_IMPL1_params_8_3_3_1600 => "NGRAM_CPS_IMPL1_params_8_3_3_1600"
-    | TABLE_BASED => "TABLE_BASED"
-    | NORMAL_FORM_TABLE_BASED => "NORMAL_FORM_TABLE_BASED"
+    | NGRAM_CPS_LRU_params_2_2_10000 => "NGRAM_CPS_LRU_params_2_2_10000"
+    | NGRAM_CPS_IMPL1_params_10_4_4_10000 => "NGRAM_CPS_IMPL1_params_10_4_4_10000"
+    | REPWL_params_4_3_320_10000 => "REPWL_params_4_3_320_10000"
     end.
 
 Definition tmAndStatusAndDeciderToString tnf_node decider_id b  :=
 tmToString (unmakeTM tnf_node.(TNF_tm)) ++ "," ++ (if (b : bool) then "halt" else "nonhalt") ++ "," ++ (deciderIdentifierToString decider_id).
 
-Redirect "BB5_Extraction/printers" Recursive Extraction tmAndStatusAndDeciderToString.
+Redirect "BB4_Extraction/printers" Recursive Extraction tmAndStatusAndDeciderToString.
 
 (**
 This is the crucial part of the extraction where we insert the print statements to print 
@@ -100,7 +88,7 @@ each enumerated machine and whether it halts or not given the conclusion reached
 
 Prints statements are inserted in place of "node_halt" and "node_nonhalt" definitions of the Coq proof, see TNF.v.
 
-In the OCaml code 'Obj.magic' is used to cast between identical types that are both defined in the 'printers' and 'bb5_verified_enumeration' files.
+In the OCaml code 'Obj.magic' is used to cast between identical types that are both defined in the 'printers' and 'BB4_verified_enumeration' files.
 **)
 
 Extract Constant node_halt => "
@@ -115,4 +103,4 @@ fun h decider_id a ->
   a
 ".
 
-Redirect "BB5_Extraction/BB5_verified_enumeration" Recursive Extraction q_200. 
+Redirect "BB4_Extraction/BB4_verified_enumeration" Recursive  Extraction q_200_def. 
