CoqBB5/BB4/BB4_TNF_Enumeration.v
@@ -1,0 +1,198 @@
+Require Import Lia.
+Require Import List.
+Require Import ZArith.
+
+From CoqBB4 Require Import TNF.
+From CoqBB4 Require Import TM.
+From CoqBB4 Require Import Deciders_Common.
+From CoqBB4 Require Import Tactics.
+From CoqBB4 Require Import BB4_Encodings.
+From CoqBB4 Require Import Prelims.
+From CoqBB4 Require Import BB4_Statement.
+From CoqBB4 Require Import BB4_Deciders_Pipeline.
+
+Definition TM0: TM Σ :=
+  fun x i => None.
+
+Definition root := {| TNF_tm:=TM0; TNF_cnt:=CountHaltTrans (TM0); TNF_ptr:=St1 |}.
+Definition root_q := SearchQueue_init root.
+
+Definition root_q_upd1:=
+  (SearchQueue_upd root_q (MakeHaltDeciderWithIdentifier decider2)).
+
+Definition first_trans_is_R(x:TNF_Node):bool :=
+  match x.(TNF_tm) St0 Σ0 with
+  | Some {| nxt:=_; dir:=Dpos; out:=_ |} => true
+  | _ => false
+  end.
+
+Definition root_q_upd1_simplified:SearchQueue:=
+  (filter first_trans_is_R (fst root_q_upd1), nil).
+
+Definition q_0 := root_q_upd1_simplified.
+Definition q_suc:SearchQueue->SearchQueue := (fun x => SearchQueue_upds x decider_all 13).
+Definition q_200_def := Nat.iter 200 q_suc q_0.
+Definition q_200 : SearchQueue := Eval native_compute in q_200_def.
+
+
+
+
+Lemma UnusedState_TM0 s1:
+  UnusedState TM0 s1 <->
+  s1 <> St0.
+Proof.
+split; intro.
+- intro H0. subst.
+  destruct H as [H [H0 H1]].
+  contradiction.
+- repeat split; auto 1.
+Qed.
+
+Lemma root_WF: TNF_Node_WF root.
+Proof.
+  repeat split.
+  1: cbn; cg.
+  unfold UnusedState_ptr.
+  left.
+  intros.
+  rewrite UnusedState_TM0.
+  destruct s0; unfold St_le; cbn; split; intro; cg; lia.
+Qed.
+
+Lemma root_q_WF:
+  SearchQueue_WF (N.to_nat BB4_minus_one) root_q root.
+Proof.
+  apply SearchQueue_init_spec,root_WF.
+Qed.
+
+Lemma root_q_upd1_WF:
+  SearchQueue_WF (N.to_nat BB4_minus_one) root_q_upd1 root.
+Proof.
+  apply SearchQueue_upd_spec.
+  - apply root_q_WF.
+  - apply decider2_WF.
+Qed.
+
+Lemma TM_rev_upd'_TM0 s0 o0:
+  (TM_upd' (TM0) St0 Σ0 (Some {| nxt := s0; dir := Dneg; out := o0 |})) =
+  (TM_rev Σ (TM_upd' (TM0) St0 Σ0 (Some {| nxt := s0; dir := Dpos; out := o0 |}))).
+Proof.
+  repeat rewrite TM_upd'_spec.
+  fext. fext.
+  unfold TM_upd,TM_rev,TM0.
+  St_eq_dec x St0.
+  - Σ_eq_dec x0 Σ0; cbn; reflexivity.
+  - cbn; reflexivity.
+Qed.
+
+Lemma root_q_upd1_simplified_WF:
+  SearchQueue_WF (N.to_nat BB4_minus_one) root_q_upd1_simplified root.
+Proof.
+  pose proof (root_q_upd1_WF).
+  cbn in H.
+  destruct H as [Ha Hb].
+  cbn.
+  split.
+  - intros x H0.
+    pose proof (Ha x). tauto.
+  - intro H0. apply Hb.
+    intros x H1.
+    destruct H1 as [H1|[H1|[H1|[H1|[H1|[H1|[H1|[H1|H1]]]]]]]]; try (specialize (H0 x); tauto).
+    1,2,3,4:
+      clear Ha; clear Hb;
+      destruct x as [tm cnt ptr];
+      cbn; invst H1;
+      rewrite TM_rev_upd'_TM0;
+      eapply HaltTimeUpperBound_LE_rev_InitES.
+    1: eassert (H2:_) by (apply (H0 {|
+             TNF_tm := TM_upd' (TM0) St0 Σ0 (Some {| nxt := St0; dir := Dpos; out := Σ0 |});
+             TNF_cnt := 7;
+             TNF_ptr := St1
+           |}); tauto); apply H2.
+    1: eassert (H2:_) by (apply (H0 {|
+             TNF_tm := TM_upd' (TM0) St0 Σ0 (Some {| nxt := St0; dir := Dpos; out := Σ1 |});
+             TNF_cnt := 7;
+             TNF_ptr := St1
+           |}); tauto); apply H2.
+    1: eassert (H2:_) by (apply (H0 {|
+             TNF_tm := TM_upd' (TM0) St0 Σ0 (Some {| nxt := St1; dir := Dpos; out := Σ0 |});
+             TNF_cnt := 7;
+             TNF_ptr := St2
+           |}); tauto); apply H2.
+    1: eassert (H2:_) by (apply (H0 {|
+             TNF_tm := TM_upd' (TM0) St0 Σ0 (Some {| nxt := St1; dir := Dpos; out := Σ1 |});
+             TNF_cnt := 7;
+             TNF_ptr := St2
+           |}); tauto); apply H2.
+Qed.
+
+Lemma q_200_spec: q_200 = Nat.iter 200 q_suc q_0.
+Proof.
+  assert (q_200 = q_200_def) as H  by (native_cast_no_check (eq_refl q_200)).
+  rewrite H. unfold q_200_def. reflexivity.
+Qed.
+
+Lemma iter_S{A}(f:A->A)(x x0:A) n:
+  x0 = Nat.iter n f x ->
+  f x0 = Nat.iter (S n) f x.
+Proof.
+  intro H.
+  rewrite H.
+  reflexivity.
+Qed.
+
+Lemma q_200_WF:
+  SearchQueue_WF (N.to_nat BB4_minus_one) q_200 root.
+Proof.
+  rewrite q_200_spec.
+  generalize 200.
+  intro n.
+  induction n.
+  - replace (Nat.iter 0 q_suc q_0) with q_0 by reflexivity.
+    unfold q_0,root_q.
+    apply root_q_upd1_simplified_WF.
+  - replace (Nat.iter (S n) q_suc q_0) with (q_suc (Nat.iter n q_suc q_0)) by (apply iter_S; reflexivity).
+    remember (Nat.iter n q_suc q_0) as q.
+    clear Heqq.
+    unfold q_suc.
+    apply SearchQueue_upds_spec.
+    + apply IHn.
+    + apply decider_all_spec.
+Qed.
+
+Lemma q_200_empty:
+  q_200 = (nil,nil).
+Proof.
+  reflexivity.
+Qed.
+
+Lemma root_HTUB:
+  TNF_Node_HTUB (N.to_nat BB4_minus_one) root.
+Proof.
+  epose proof q_200_WF.
+  unfold SearchQueue_WF in H.
+  rewrite q_200_empty in H.
+  apply H.
+  cbn.
+  intros.
+  contradiction.
+Qed.
+
+Lemma TM0_HTUB:
+  HaltTimeUpperBound Σ (N.to_nat BB4_minus_one) (InitES Σ Σ0) (LE Σ (TM0)).
+Proof.
+  apply root_HTUB.
+Qed.
+
+Lemma allTM_HTUB:
+  HaltTimeUpperBound Σ (N.to_nat BB4_minus_one) (InitES Σ Σ0) (fun _ => True).
+Proof.
+  unfold HaltTimeUpperBound.
+  intros.
+  eapply TM0_HTUB.
+  2: apply H0.
+  unfold LE.
+  intros.
+  right.
+  reflexivity.
+Qed.
