CoqBB5/BB4/Deciders/Decider_Halt_BB4.v
@@ -1,0 +1,17 @@
+Require Import Lia.
+Require Import ZArith.
+
+From CoqBB4 Require Import TM.
+From CoqBB4 Require Import BB4_Statement.
+From CoqBB4 Require Import BB4_Encodings.
+From CoqBB4 Require Import Deciders_Common.
+From CoqBB4 Require Import Decider_Halt.
+
+Set Warnings "-abstract-large-number".
+
+Definition halt_decider_max := halt_decider 106.
+Lemma halt_decider_max_spec: HaltDecider_WF (N.to_nat BB4_minus_one) halt_decider_max.
+Proof.
+  eapply halt_decider_WF.
+  unfold BB4_minus_one. lia.
+Qed.
