CoqBB5/BB4/BB4_Extraction/BB4_Extraction.sh
@@ -1,5 +1,5 @@
 cp printers.out printers.ml
-cp BB2x4_verified_enumeration.out BB2x4_verified_enumeration.ml
+cp BB4_verified_enumeration.out BB4_verified_enumeration.ml
 
 # We need high stack size for compiling the OCaml extraction
 # Get the hard limit for stack size
@@ -14,7 +14,7 @@ echo "Stack size limit: $(ulimit -S -s)"
 
 echo "Compiling extraction..."
 
-ocamlbuild BB2x4_verified_enumeration.native -pkg zarith
+ocamlbuild BB4_verified_enumeration.native -pkg zarith
 
 if [ $? -ne 0 ]; then  # Check if the command failed
     echo ""
@@ -27,33 +27,33 @@ if [ $? -ne 0 ]; then  # Check if the command failed
 fi
 
 echo "Extraction compiled with success"
-echo "Running extraction, see generated 'BB2x4_verified_enumeration.csv'..."
+echo "Running extraction, see generated 'BB4_verified_enumeration.csv'..."
 
-echo "machine,status,decider" > BB2x4_verified_enumeration.csv
-./BB2x4_verified_enumeration.native >> BB2x4_verified_enumeration.csv
+echo "machine,status,decider" > BB4_verified_enumeration.csv
+./BB4_verified_enumeration.native >> BB4_verified_enumeration.csv
 
 # Remove empty trailing line
-printf "%s" "$(< BB2x4_verified_enumeration.csv)" > tmp
-mv tmp BB2x4_verified_enumeration.csv
+printf "%s" "$(< BB4_verified_enumeration.csv)" > tmp
+mv tmp BB4_verified_enumeration.csv
 
-echo "BB2x4 extraction done!"
+echo "BB4 extraction done!"
 
 if command -v sha256sum &> /dev/null; then
-    ACTUAL_HASH=$(sha256sum "BB2x4_verified_enumeration.csv" | awk '{print $1}')
+    ACTUAL_HASH=$(sha256sum "BB4_verified_enumeration.csv" | awk '{print $1}')
 elif command -v shasum &> /dev/null; then
-    ACTUAL_HASH=$(shasum -a 256 "BB2x4_verified_enumeration.csv" | awk '{print $1}')
+    ACTUAL_HASH=$(shasum -a 256 "BB4_verified_enumeration.csv" | awk '{print $1}')
 else
     echo "Error: No SHA-256 hashing tool found."
     exit 1
 fi
 
-EXPECTED_HASH=0b8aba94937522eda0995a549fa2e2d86d2a5b8f9cc66e5c0a1500dbbe59a814
+EXPECTED_HASH=c517de277a3f0c8c95ffefa510caf834d8f53763e59623813f98c2b64c6df621
 # Compare the hashes
 if [[ "$ACTUAL_HASH" == "$EXPECTED_HASH" ]]; then
-    echo "Success: Hash matches the expected one from BB2x4 extraction."
+    echo "Success: Hash matches the expected one from BB4 extraction."
     exit 0
 else
-    echo "Error: Hash does not match the expected one from BB2x4 extraction."
+    echo "Error: Hash does not match the expected one from BB4 extraction."
     echo "Expected: $EXPECTED_HASH"
     echo "Actual:   $ACTUAL_HASH"
     exit 1
